Foundation/Propositional/Kripke/Hilbert/LC.lean
@@ -1,7 +1,6 @@
 import Foundation.Propositional.Hilbert.WellKnown
-import Foundation.Propositional.Kripke.Hilbert.Soundness
-import Foundation.Propositional.Kripke.Completeness
 import Foundation.Propositional.Kripke.AxiomDummett
+import Foundation.Propositional.Kripke.Hilbert.Soundness
 
 namespace LO.Propositional
 
@@ -10,17 +9,16 @@ open Formula.Kripke
 
 namespace Hilbert.LC.Kripke
 
-instance : ConnectedFrameClass.DefinedBy (Hilbert.LC.axioms) := FrameClass.definedBy_with_axiomEFQ inferInstance
+instance : FrameClass.connected.DefinedBy (Hilbert.LC.axioms) := FrameClass.definedBy_with_axiomEFQ inferInstance
 
-instance sound : Sound Hilbert.LC ConnectedFrameClass := inferInstance
+instance sound : Sound Hilbert.LC FrameClass.connected := inferInstance
 
-instance consistent : Entailment.Consistent Hilbert.LC := Kripke.Hilbert.consistent_of_FrameClass ConnectedFrameClass
+instance consistent : Entailment.Consistent Hilbert.LC := Kripke.Hilbert.consistent_of_FrameClass FrameClass.connected (by simp)
 
-instance canonical : Canonical Hilbert.LC ConnectedFrameClass := ⟨Canonical.connected⟩
+instance canonical : Canonical Hilbert.LC FrameClass.connected := ⟨Canonical.connected⟩
 
-instance complete : Complete Hilbert.LC ConnectedFrameClass := inferInstance
+instance complete : Complete Hilbert.LC FrameClass.connected := inferInstance
 
 end Hilbert.LC.Kripke
-
 
 end LO.Propositional
