Foundation/Propositional/Logic/Basic.lean
@@ -55,10 +55,7 @@ open Kripke
 
 abbrev Kripke.FrameClass.logic (C : FrameClass) : Logic := { φ | C ⊧ φ }
 
-abbrev Kripke.FiniteFrameClass.logic (C : FiniteFrameClass) : Logic := { φ | C ⊧ φ }
-
-lemma Logic.eq_Hilbert_Logic_KripkeFrameClass_Logic
-  {H : Hilbert ℕ} {C : FrameClass}
+lemma Logic.eq_Hilbert_Logic_KripkeFrameClass_Logic {H : Hilbert ℕ} {C : FrameClass}
   [sound : Sound H C] [complete : Complete H C]
   : H.logic = C.logic := by
   ext φ;
@@ -66,18 +63,9 @@ lemma Logic.eq_Hilbert_Logic_KripkeFrameClass_Logic
   . exact sound.sound;
   . exact complete.complete;
 
-lemma Logic.eq_Hilbert_Logic_KripkeFiniteFrameClass_Logic
-  {H : Hilbert ℕ} {C : FiniteFrameClass}
-  [sound : Sound H C] [complete : Complete H C]
-  : H.logic = C.logic := by
-  ext φ;
-  constructor;
-  . exact sound.sound;
-  . exact complete.complete;
+lemma Logic.Int.Kripke.eq_all : Logic.Int = FrameClass.all.logic := eq_Hilbert_Logic_KripkeFrameClass_Logic
 
-lemma Logic.Int.eq_AllKripkeFrameClass_Logic : Logic.Int = AllFrameClass.logic := eq_Hilbert_Logic_KripkeFrameClass_Logic
-
-lemma Logic.Int.eq_AllFiniteKripkeFrameClass_Logic : Logic.Int = AllFiniteFrameClass.logic := eq_Hilbert_Logic_KripkeFiniteFrameClass_Logic
+lemma Logic.Int.Kripke.eq_all_finite : Logic.Int = Kripke.FrameClass.all_finite.logic := eq_Hilbert_Logic_KripkeFrameClass_Logic
 
 end
 
