Foundation/Propositional/Logic/Sublogic.lean
@@ -9,11 +9,11 @@ open Formula.Kripke
 theorem Int_ssubset_KC : Logic.Int ⊂ Logic.KC := by
   constructor;
   . exact (Hilbert.weakerThan_of_subset_axioms (by simp)).subset;
-  . suffices ∃ φ, Hilbert.KC ⊢! φ ∧ ¬AllFrameClass ⊧ φ by simpa [Int.eq_AllKripkeFrameClass_Logic];
+  . suffices ∃ φ, Hilbert.KC ⊢! φ ∧ ¬FrameClass.all ⊧ φ by simpa [Int.Kripke.eq_all]
     use Axioms.WeakLEM (.atom 0);
     constructor;
     . exact wlem!;
-    . apply Formula.Kripke.ValidOnFrameClass.not_of_exists_frame;
+    . apply Kripke.validOnFrameClass_not_of_exists_frame;
       let F : Frame := {
         World := Fin 3
         Rel := λ x y => x = 0 ∨ (x = y)
@@ -25,7 +25,7 @@ theorem Int_ssubset_KC : Logic.Int ⊂ Logic.KC := by
       constructor;
       . tauto;
       . apply (show ¬Confluent F.Rel → ¬ValidOnFrame F (Axioms.WeakLEM (.atom 0)) by
-          simpa using Kripke.ConfluentFrameClass.DefinedByAxiomWeakLEM.defines F |>.not.mp
+          simpa using FrameClass.confluent.definability.defines F |>.not.mp
         );
         unfold Confluent;
         push_neg;
@@ -36,11 +36,11 @@ theorem KC_ssubset_LC : Logic.KC ⊂ Logic.LC := by
   constructor;
   . exact (Hilbert.weakerThan_of_dominate_axiomInstances
       (by rintro _ ⟨ψ, ⟨(rfl | rfl), ⟨s, rfl⟩⟩⟩ <;> simp [efq!, wlem!])).subset
-  . suffices ∃ φ, Hilbert.LC ⊢! φ ∧ ¬ConfluentFrameClass ⊧ φ by simpa [KC.eq_ConfluentKripkeFrameClass_Logic];
+  . suffices ∃ φ, Hilbert.LC ⊢! φ ∧ ¬FrameClass.confluent ⊧ φ by simpa [KC.Kripke.eq_confluent];
     use Axioms.Dummett (.atom 0) (.atom 1);
     constructor;
     . exact dummett!;
-    . apply Formula.Kripke.ValidOnFrameClass.not_of_exists_frame;
+    . apply Kripke.validOnFrameClass_not_of_exists_frame;
       let F : Frame := {
         World := Fin 4
         Rel := λ x y => ¬(x = 1 ∧ y = 2) ∧ ¬(x = 2 ∧ y = 1) ∧ (x ≤ y)
@@ -55,7 +55,7 @@ theorem KC_ssubset_LC : Logic.KC ⊂ Logic.LC := by
         use 3;
         omega;
       . apply (show ¬Connected F.Rel → ¬ValidOnFrame F (Axioms.Dummett (.atom 0) (.atom 1)) by
-          simpa using Kripke.ConnectedFrameClass.DefinedByAxiomDummett.defines F |>.not.mp
+          simpa using FrameClass.connected.definability.defines F |>.not.mp
         );
         unfold Connected;
         push_neg;
@@ -66,11 +66,11 @@ theorem LC_ssubset_Cl : Logic.LC ⊂ Logic.Cl := by
   constructor;
   . apply (Hilbert.weakerThan_of_dominate_axiomInstances
       (by rintro _ ⟨ψ, ⟨(rfl | rfl), ⟨s, rfl⟩⟩⟩ <;> simp [efq!, dummett!])).subset;
-  . suffices ∃ φ, Hilbert.Cl ⊢! φ ∧ ¬ConnectedFrameClass ⊧ φ by simpa [LC.eq_ConnectedKripkeFrameClass_Logic];
+  . suffices ∃ φ, Hilbert.Cl ⊢! φ ∧ ¬FrameClass.connected ⊧ φ by simpa [LC.Kripke.eq_connected];
     use Axioms.LEM (.atom 0);
     constructor;
     . exact lem!;
-    . apply Formula.Kripke.ValidOnFrameClass.not_of_exists_frame;
+    . apply Kripke.validOnFrameClass_not_of_exists_frame;
       let F : Frame := {
         World := Fin 2,
         Rel := λ x y => x ≤ y
@@ -82,7 +82,7 @@ theorem LC_ssubset_Cl : Logic.LC ⊂ Logic.Cl := by
       constructor;
       . simp [F, Connected]; omega;
       . apply (show ¬Euclidean F.Rel → ¬ValidOnFrame F (Axioms.LEM (.atom 0)) by
-          simpa using Kripke.EuclideanFrameClass.DefinedByAxiomLEM.defines F |>.not.mp
+          simpa using FrameClass.euclidean.definability.defines F |>.not.mp
         );
         unfold Euclidean;
         push_neg;
